Turned ltl2omega.sml into a selftest

examples/temporal_deep/src/examples/ltl2omega.sml
@@ -7,6 +7,8 @@ open full_ltlTheory arithmeticTheory automaton_formulaTheory xprop_logicTheory p
      rltl_to_ltlTheory psl_to_rltlTheory UnclockedSemanticsTheory
      SyntacticSugarTheory congLib temporal_deep_simplificationsLib;
 
+open testutils;
+
 (* A function to generate test ltl formulas.
    This has been kindly provided by Kristin Yvonne Rozier <kyrozier@cs.rice.edu>
 
@@ -14,7 +16,6 @@ open full_ltlTheory arithmeticTheory automaton_formulaTheory xprop_logicTheory p
    Output: an LTL formula describing an n-bit counter
  *)
 local
-
   fun mpattern_int 0 = ``LTL_NEXT (m:'a ltl)``
     | mpattern_int n = subst [mk_var ("X", ``:'a ltl``) |-> mpattern_int (n-1)]
                           ``LTL_NEXT (LTL_AND(LTL_NOT (m:'a ltl), X))``;
@@ -78,21 +79,18 @@ in
     in
       term
     end
-
 end;
 
 val pslTerm = ``
-    F_ALWAYS (F_IMPLIES(F_STRONG_BOOL (B_PROP aa),
-                    F_STRONG_NEXT_EVENT (B_PROP bb,
-                                         F_STRONG_BEFORE (
+    F_ALWAYS (F_IMPLIES (
+                 F_STRONG_BOOL (B_PROP aa),
+                 F_STRONG_NEXT_EVENT (B_PROP bb,
+                                      F_STRONG_BEFORE (
                                             F_STRONG_BOOL (B_PROP cc),
-                                            F_STRONG_BOOL (B_PROP dd)
-                                         ))
-                   )
-         )``;
-
+                                            F_STRONG_BOOL (B_PROP dd)))))``;
 
 val rltlTerm = (liteLib.mk_icomb (``PSL_TO_RLTL``, pslTerm));
+
 val rltlTermEval = rhs (concl (
 SIMP_CONV std_ss [PSL_TO_RLTL_def, F_ALWAYS_def, F_G_def,
                   F_F_def, BEXP_TO_PROP_LOGIC_def,
@@ -106,9 +104,8 @@ val ltlTermEval = rhs (concl (
 val ltlTermSimp = rand ( concl (
   CONGRUENCE_SIMP_CONV ``LTL_EQUIVALENT`` ltl_nnf_cs std_ss [] ltlTermEval))
 
-(*Example from "Construction Buechi Automata from Linear Temporal Logic Using
-   Simulation Relations for Alternating Buechi Automata" by Carsten Fritz*)
-
+(* Example from "Construction Buechi Automata from Linear Temporal Logic Using
+   Simulation Relations for Alternating Buechi Automata" by Carsten Fritz *)
 val test0LTL = ``
     LTL_NOT
      (LTL_SUNTIL (LTL_SUNTIL (LTL_NEXT (LTL_PROP (P_PROP b)),
@@ -156,26 +153,151 @@ val test15LTL = ``LTL_SUNTIL (LTL_PROP (P_PROP p), LTL_PROP (P_PROP q))``;
 val test1RLTL = ``RLTL_PROP (P_PROP a)``;
 val test2RLTL = ``RLTL_NOT(RLTL_PROP (P_PROP (a:'c)))``;
 val test3RLTL = ``RLTL_ACCEPT (RLTL_SUNTIL (RLTL_PROP (P_PROP a),
-                                            RLTL_NEXT (RLTL_PROP (P_PROP a))),
-                               P_PROP c)``;
+                                            RLTL_NEXT (RLTL_PROP (P_PROP a))), P_PROP c)``;
 
-(*Some examples to execute at interactivly. Just change the
-  number of the test terms or introduce on terms *)
+(* Some examples to execute at interactivly. Just change the
+   number of the test terms or introduce on terms
+
+   syntax: ltl2omega fast neg ltl *)
+
+fun ltl2omega_test (test_fn, problem, result) = let
+    val _ = tprint (term_to_string problem);
+in
+    require (check_result (aconv result o concl)) test_fn problem
+end;
+
+val test_cases =
+   [(ltl2omega false (* no-fast *) false (* orig *), test15LTL (* p U q *),
+     ``!sv.
+          IS_ELEMENT_ITERATOR sv 1 {q; p} ==>
+          !i.
+              LTL_SEM i
+                (LTL_SUNTIL (LTL_PROP (P_PROP p),LTL_PROP (P_PROP q))) <=>
+              A_SEM i
+                (A_UNIV
+                   (symbolic_semi_automaton (\s. ?n. n < 1 /\ s = sv n)
+                      (P_BIGAND [])
+                      (XP_BIGAND
+                         [XP_EQUIV
+                            (XP_PROP (sv 0),
+                             XP_OR
+                               (XP_PROP q,
+                                XP_AND (XP_PROP p,XP_NEXT_PROP (sv 0))))]),
+                    A_IMPL (A_BIGAND [],ACCEPT_COND_PROP (P_PROP (sv 0)))))``),
+
+    (ltl2omega false (* no-fast *) true (* neg *), test15LTL,
+     ``!sv.
+          IS_ELEMENT_ITERATOR sv 1 {q; p} ==>
+          !i.
+              LTL_SEM i
+                (LTL_SUNTIL (LTL_PROP (P_PROP p),LTL_PROP (P_PROP q))) <=>
+              A_SEM i
+                (A_NDET
+                   (symbolic_semi_automaton (\s. ?n. n < 1 /\ s = sv n)
+                      (P_BIGAND [])
+                      (XP_BIGAND
+                         [XP_EQUIV
+                            (XP_PROP (sv 0),
+                             XP_OR
+                               (XP_PROP q,
+                                XP_AND (XP_PROP p,XP_NEXT_PROP (sv 0))))]),
+                    A_AND
+                      (A_BIGAND
+                         [ACCEPT_COND_GF (P_IMPL (P_PROP (sv 0),P_PROP q))],
+                       ACCEPT_COND_PROP (P_PROP (sv 0)))))``),
+
+    (ltl2omega true (* fast *) false (* orig *), test15LTL,
+     ``!sv.
+          IS_ELEMENT_ITERATOR sv 1 {p; q} ==>
+          !i.
+              LTL_SEM i
+                (LTL_SUNTIL (LTL_PROP (P_PROP p),LTL_PROP (P_PROP q))) <=>
+              A_SEM i
+                (A_UNIV
+                   (symbolic_semi_automaton (\s. ?n. n < 1 /\ s = sv n)
+                      (P_BIGAND [])
+                      (XP_BIGAND
+                         [XP_EQUIV
+                            (XP_PROP (sv 0),
+                             XP_OR
+                               (XP_CURRENT (P_PROP q),
+                                XP_AND
+                                  (XP_CURRENT (P_PROP p),XP_NEXT_PROP (sv 0))))]),
+                    A_IMPL (A_BIGAND [],ACCEPT_COND_PROP (P_PROP (sv 0)))))``),
+
+    (ltl2omega true (* fast *) true (* neg *), test15LTL,
+     ``!sv.
+          IS_ELEMENT_ITERATOR sv 1 {p; q} ==>
+          !i.
+              LTL_SEM i
+                (LTL_SUNTIL (LTL_PROP (P_PROP p),LTL_PROP (P_PROP q))) <=>
+              A_SEM i
+                (A_NDET
+                   (symbolic_semi_automaton (\s. ?n. n < 1 /\ s = sv n)
+                      (P_BIGAND [])
+                      (XP_BIGAND
+                         [XP_EQUIV
+                            (XP_PROP (sv 0),
+                             XP_OR
+                               (XP_CURRENT (P_PROP q),
+                                XP_AND
+                                  (XP_CURRENT (P_PROP p),XP_NEXT_PROP (sv 0))))]),
+                    A_AND
+                      (A_BIGAND
+                         [ACCEPT_COND_GF (P_IMPL (P_PROP (sv 0),P_PROP q))],
+                       ACCEPT_COND_PROP (P_PROP (sv 0)))))``),
+
+    (ltl2omega_rewrite true (* max *), test15LTL,
+     ``!sv.
+          IS_ELEMENT_ITERATOR sv 1 {p; q} ==>
+          !i.
+              LTL_SEM i
+                (LTL_SUNTIL (LTL_PROP (P_PROP p),LTL_PROP (P_PROP q))) <=>
+              A_SEM i
+                (A_NDET
+                   (symbolic_semi_automaton (\s. ?n. n < 1 /\ s = sv n)
+                      P_TRUE
+                      (XP_AND
+                         (XP_EQUIV
+                            (XP_PROP (sv 0),
+                             XP_OR
+                               (XP_PROP q,
+                                XP_AND (XP_PROP p,XP_NEXT_PROP (sv 0)))),
+                          XP_TRUE)),
+                    A_AND
+                      (A_AND
+                         (ACCEPT_COND_GF (P_IMPL (P_PROP (sv 0),P_PROP q)),
+                          A_TRUE),ACCEPT_COND_PROP (P_PROP (sv 0)))))``),
+
+    (ltl2omega_rewrite false (* min *), test15LTL,
+     ``!sv.
+          IS_ELEMENT_ITERATOR sv 1 {p; q} ==>
+          !i.
+              LTL_SEM i
+                (LTL_SUNTIL (LTL_PROP (P_PROP p),LTL_PROP (P_PROP q))) <=>
+              A_SEM i
+                (A_UNIV
+                   (symbolic_semi_automaton (\s. ?n. n < 1 /\ s = sv n)
+                      P_TRUE
+                      (XP_AND
+                         (XP_EQUIV
+                            (XP_PROP (sv 0),
+                             XP_OR
+                               (XP_PROP q,
+                                XP_AND (XP_PROP p,XP_NEXT_PROP (sv 0)))),
+                          XP_TRUE)),
+                    A_IMPL (A_TRUE,ACCEPT_COND_PROP (P_PROP (sv 0)))))``)];
+
+val _ = List.app (ignore o ltl2omega_test) test_cases;
+
+(* simplified tests, only make sure the test function has no exception *)
+fun ltl2omega_test_simple (test_fn, problem) = let
+    val _ = tprint (term_to_string problem);
+in
+    require (check_result (fn th => true)) test_fn problem
+end;
 
 (*
-
-ltl2omega false false test13LTL
-ltl2omega true  false test13LTL
-
-(* syntax: ltl2omega fast neg ltl *)
-
-ltl2omega false (* no-fast *) false (* orig *) test15LTL;
-ltl2omega false (* no-fast *) true  (* neg *)  test15LTL;
-ltl2omega true false test15LTL;
-ltl2omega true true test15LTL;
-ltl2omega_rewrite true  (* max *) test15LTL; (* p U q *)
-ltl2omega_rewrite false (* min *) test15LTL; (* p U q *)
-
 ************************************************
 The fast switch has some influence. Notice the
 different number of needed state vars and the
@@ -187,21 +309,56 @@ time (ltl2omega false true) test13LTL
 
 time (ltl2omega true true) test0LTL
 time (ltl2omega false true) test0LTL
+*)
 
+val test_cases_simple =
+   [(ltl2omega false false, test0LTL),
+    (ltl2omega true  false, test0LTL),
+    (ltl2omega false false, test1LTL),
+    (ltl2omega false false, test2LTL),
+    (ltl2omega false false, test3LTL),
+    (ltl2omega false false, test4LTL),
+    (ltl2omega false false, test5LTL),
+    (ltl2omega false false, test6LTL),
+    (ltl2omega false false, test7LTL),
+    (ltl2omega false false, test8LTL),
+    (ltl2omega false false, test9LTL),
+    (ltl2omega false false, test10LTL),
+    (ltl2omega false false, test11LTL),
+    (ltl2omega false false, test12LTL),
+    (ltl2omega false false, test13LTL),
+    (ltl2omega true  false, test13LTL)];
+
+val _ = List.app (ignore o ltl2omega_test_simple) test_cases_simple;
+
+(*
 ************************************************
 Internal view. The fast version keeps just one
 binding. The slow one keeps all
 ************************************************
-ltl2omega_internal true true test11LTL
-ltl2omega_internal false true test11LTL
 
+NOTE: val (b1, b2) = if neg then (true, false) else (false, true);
 
+ltl2omega_internal true  (* fast *) false (* b1 *) true (* b2 *) test11LTL
+ltl2omega_internal false (* slow *) false (* b1 *) true (* b2 *) test11LTL
+ *)
+
+val test_cases_simple2 =
+   [(ltl2omega_internal true  (* fast *) false (* b1 *) true (* b2 *), test11LTL),
+    (ltl2omega_internal false (* slow *) false (* b1 *) true (* b2 *), test11LTL)
+    ];
+
+val _ = List.app (ignore o ltl2omega_test_simple) test_cases_simple2;
+
+(*
 ************************************************
 A simple, non optimised translation that uses
 just rewriting. Just a proof of concept
 ************************************************
 time (ltl2omega_rewrite true) test11LTL
+ *)
 
+(*
 ************************************************
 Translations to kripke_structure
 ************************************************
@@ -215,11 +372,31 @@ time (ltl_contradiction2ks_fair_emptyness true) test13LTL
 time (ltl_contradiction2ks_fair_emptyness___num 1 true) test13LTL
 time (ltl_contradiction2ks_fair_emptyness___num 2 true) test13LTL
 time (ltl_contradiction2ks_fair_emptyness___num 3 true) test13LTL
+ *)
 
+val test_cases_simple3 =
+   [(ltl_contradiction2ks_fair_emptyness true, test11LTL),
+    (ltl_contradiction2ks_fair_emptyness true, test13LTL)];
+
+val _ = List.app (ignore o ltl2omega_test_simple) test_cases_simple3;
+
+val test_cases_simple4 =
+   [(ltl_contradiction2ks_fair_emptyness___num 1 true, test11LTL),
+    (ltl_contradiction2ks_fair_emptyness___num 2 true, test11LTL),
+    (ltl_contradiction2ks_fair_emptyness___num 3 true, test11LTL),
+    (ltl_contradiction2ks_fair_emptyness___num 1 true, test13LTL),
+    (ltl_contradiction2ks_fair_emptyness___num 2 true, test13LTL),
+    (ltl_contradiction2ks_fair_emptyness___num 3 true, test13LTL)];
+
+val _ = List.app (ignore o ltl2omega_test_simple) test_cases_simple4;
+
+(*
 val ltl_ks_sem2ks_fair_emptyness___no_ks : bool -> term -> thm
 val ltl_ks_sem2ks_fair_emptyness : bool -> term -> term -> thm
 val ltl_equivalent2ks_fair_emptyness : bool -> term -> term -> thm
+ *)
 
+(*
 *************************************************
 LTL counters
 These can be used to test performance on
@@ -227,9 +404,18 @@ huge formulas. Additionally these formulas contain
 large subterms several times. Thus they benefit from
 using the "slow" version
 *************************************************
+
 time (ltl2omega false true) (ltl_counter 2)
 time (ltl2omega true true) (ltl_counter 2)
+ *)
 
+val test_cases_ltl_counter =
+   [(ltl2omega false true, ltl_counter 2),
+    (ltl2omega true  true, ltl_counter 2)];
+
+val _ = List.app (ignore o ltl2omega_test_simple) test_cases_ltl_counter;
+
+(*
 ************************************************
 You may also be interested in the following
 definitions and theorems
@@ -246,5 +432,6 @@ LTL_TO_GEN_BUECHI_DS___FAIR_RUN_def
 LTL_TO_GEN_BUECHI_DS___BINDING_RUN_def
 LTL_TO_GEN_BUECHI_DS___MIN_FAIR_RUN_def
 LTL_TO_GEN_BUECHI_DS___MAX_FAIR_RUN_def
-
 *)
+
+val _ = Process.exit Process.success;
